% уравнение один
\def \equationFirst {x{y}' \cdot \ln{x} - y = 3x^2 \cdot \ln^{2}{x}}
\def \conditionFirst {y(\sqrt[3]{e}) = 0}
\newcommand{\solutionFirst}[1][C] {y = \dfrac{3x^2\ln{x}}{2} + #1\ln{x}}
\def \constantFirst {\dfrac{3 e^{\frac{2}{3}}}{2}}

% уравнение два
\def \equationSecond {{y}' \cdot \ln{x} + 2xy = 2x \cdot \sqrt{y}}
\def \conditionSecond {y(0) = 1}
\newcommand{\solutionSecond}[1][C] {\ln{\sqrt{y} - 1} = #1 - \Ei{2\ln{x}}}
\def \constantSecond {-1}

\newcommand{\taskTwoSolutionItem}[5]{
	\item 
		$ #1 $ % #1 - уравнение
	
	\textit{Общее решение}: 
		$ #2, \ {C} \in \rational $ % #2 - общее решение
	
	Подставим $ #3 $ в общее решение: % #3 - условие
	
	$ C = #4 $ % #4 - найденное С
	
	\answer $ \displaystyle #5 $ % #5 - ответ
}
